Earley/Proofs/Parser.lean
@@ -166,6 +166,92 @@ public theorem correctnessParse {G : ContextFreeGrammar T} [BEq G.NT] [LawfulBEq
     G.Generates (mapT w) ↔ ∃ t, parse Gₗ w = some t := by
   grind [soundnessParse, completenessParse]
 
+-- TODO: move these somewhere else
+/--
+Returns the terminals stored within the parse tree.
+-/
+def yield : (Tree T N) → List T
+| Tree.leaf (Symbol.nonterminal _) => []
+| Tree.leaf (Symbol.terminal t) => [t]
+| Tree.node _ ts => (ts.map yield).flatten
+
+def root : (Tree T N) → Symbol T N
+| Tree.leaf d => d
+| Tree.node d _ => d
+
+/--
+Each node of the tree has to correspond to a rule of the grammar.
+-/
+def wfRuleTree (G : ContextFreeGrammarList T N) : Tree T N → Prop
+| Tree.leaf _ => True
+| Tree.node d ts => (∃ r ∈ G.rules, d = Symbol.nonterminal r.input ∧ (ts.map root = r.output))
+  ∧ (∀ t ∈ ts, wfRuleTree G t)
+
+/--
+Each node of the tree has to correspond to an item of the grammar.
+-/
+def wfItemTree (G : ContextFreeGrammarList T N) (x : EarleyItem T N) : Tree T N → Prop
+| Tree.leaf _ => True
+| Tree.node d ts =>
+  (d = Symbol.nonterminal x.rule.input ∧ (ts.map root = x.rule.output.take x.position))
+  ∧ (∀ t ∈ ts, wfRuleTree G t)
+
+/--
+The tree of an item is well-formed w.r.t. to yield iff it parses what it claims to parse.
+-/
+def wfYield (w : List T) (x : EarleyItem T N) (t : Tree T N) : Prop :=
+  yield t = slice w x.startIdx x.endIdx
+
+lemma yieldBuildTree_eq_word {G : ContextFreeGrammarList T N} {w : Array T} (j k : Nat)
+    {bins : EarleyBins T N (w.size + 1)} (hbins : EarleyBins.WF G bins)
+    (hwf : EarleyBins.PointerWF bins) (hk : k < w.size + 1)
+    (hj : j < bins[k].length) (hw : w ≠ #[])
+    {t : Tree T N} (ht : buildTree G w hw bins hbins hwf k hk j hj = some t) :
+    wfYield w.toList bins[k][j].item t := by
+  fun_induction buildTree G w hw bins hbins hwf k hk j hj with
+  | case1 k hk j hj x hpx =>
+    simp [wfYield]
+    simp at ht
+    simp [← ht, yield]
+    sorry -- predicts
+  | case2 k hk j hj x i hpx hk2 ih =>
+    sorry
+  | case3 k hk j hj x endIdxA i j' ps hpx inv ih1 ih2 =>
+    sorry
+
+-- TODO: if I manage, also extend it to cached : )
+public theorem yieldParse_eq_word {G : ContextFreeGrammar T} [BEq G.NT] [LawfulBEq G.NT]
+    [LawfulBEq (EarleyItem T G.NT)] (w : Array T) {Gₗ : ContextFreeGrammarList T G.NT}
+    (h : CFGEqCFGₗ G Gₗ) (heps : isEpsilonFree G) {t : Tree T G.NT} (ht : parse Gₗ w = some t) :
+    -- wf_rule_tree G t
+    root t = Symbol.nonterminal Gₗ.initial
+    ∧ yield t = w.toList := by
+  simp only [parse, Option.dite_none_left_eq_some] at ht
+  rcases ht with ⟨hnEmpty, ht⟩
+  split at ht
+  · simp at ht
+  · rename_i x j _ heq
+    let finalBin := (earleyList Gₗ w).bins[w.size]
+    let P := fun x : BinItem T G.NT => isFinished Gₗ.initial w.size x.item
+    have hmem : (x, j) ∈ (filterWithIdx finalBin P) := by grind
+    have hfin := P_of_filterWithIdx (earleyList Gₗ w).bins[w.size] P hmem
+    have hj : j < List.length finalBin := by grind
+    have hx : (earleyList Gₗ w).bins[w.size][j].item = x.item := by
+      have := getElem_of_filterWithIdx finalBin P hmem
+      grind
+    --have : (hwf : EarleyBins.PointerWF bins)  :=
+    have hwf := pointerWF_of_earleyList Gₗ w
+    have h := yieldBuildTree_eq_word j w.size (earleyList Gₗ w).inv hwf (by lia) hj hnEmpty ht
+    simp only [wfYield, hx] at h
+    simp only [isFinished, Bool.and_eq_true, beq_iff_eq, P] at hfin
+
+    have : x.item.startIdx = 0 ∧ x.item.endIdx = w.toList.length := by grind
+    refine ⟨?_, by grind⟩
+    simp [root]
+    have : x.item.rule.input = Gₗ.initial := by grind
+    -- line 1185, requires wf_rule_tree and wf_item_tree
+    sorry
+
 end Naive
 
 section Cached
@@ -188,7 +274,7 @@ public theorem parseCached_eq_parse {G : ContextFreeGrammarList T N} (w : Array 
   grind
 
 /--
-A refinement proof for the the same algorithm, but utilizing a cached implementation
+A refinement proof of correctness for the the same algorithm, but utilizing a cached implementation
 to compute the bins.
 -/
 public theorem correctnessCachedParse {G : ContextFreeGrammar T} [BEq G.NT] [LawfulBEq G.NT]
@@ -196,6 +282,18 @@ public theorem correctnessCachedParse {G : ContextFreeGrammar T} [BEq G.NT] [Law
     {Gₗ : ContextFreeGrammarList T G.NT} (h : CFGEqCFGₗ G Gₗ) (heps : isEpsilonFree G) :
     G.Generates (mapT w) ↔ ∃ t, parseCached Gₗ w = some t := by
   grind [parseCached_eq_parse, correctnessParse]
+
+/--
+A refinement proof of yiled for the the same algorithm, but utilizing a cached implementation
+to compute the bins.
+-/
+public theorem yieldCachedParse_eq_word {G : ContextFreeGrammar T} [BEq G.NT] [LawfulBEq G.NT]
+    [LawfulBEq (EarleyItem T G.NT)] [Hashable G.NT] [Hashable (EarleyItem T G.NT)] (w : Array T)
+    {Gₗ : ContextFreeGrammarList T G.NT} (h : CFGEqCFGₗ G Gₗ) (heps : isEpsilonFree G)
+    {t : Tree T G.NT} (ht : parseCached Gₗ w = some t) :
+    -- wf_rule_tree G t -- TODO: if I manage, also extend it to cached : )
+    root t = Symbol.nonterminal Gₗ.initial ∧ yield t = w.toList := by
+  grind [parseCached_eq_parse, yieldParse_eq_word]
 
 end Cached
 
